\documentclass[12pt]{mwart}
\usepackage[utf8]{inputenc}
\usepackage[T1]{fontenc}
\usepackage{mathtools, amsthm, amssymb}
\usepackage[a4paper, vmargin=2.5cm, hmargin=2.5cm]{geometry}
\usepackage{colortbl}
\usepackage{hyperref}
\usepackage{xcolor}
\usepackage[makeroom]{cancel}
\usepackage{tikz}
\usepackage{scalerel}
\usepackage{pict2e}
\usepackage{tkz-euclide}
\usepackage{enumitem}
\usetikzlibrary{shapes}
\usepackage{color,xcolor}
\usepackage{soul}
\usepackage{pifont}
\usepackage{bm}
\usepackage{pgfplots}
\pgfplotsset{compat=newest}
\usepgfplotslibrary{statistics}
\usepgfplotslibrary{fillbetween}
\usetikzlibrary{calc}
\usetikzlibrary{patterns, arrows.meta}
\usetikzlibrary{shadows}
\usetikzlibrary{external}
\DeclareMathOperator{\tg}{\text{tg}}
\DeclareMathOperator{\ctg}{\text{ctg}}
\DeclareMathOperator{\e}{\text{e}}
\DeclareMathOperator{\MAD}{\text{MAD}}
\DeclareMathOperator{\IQR}{\text{IQR}}
\mathtoolsset{showonlyrefs, mathic}
\usepackage[plmath]{polski}
\author{Piotr Zieleń}
\title{Matematyka dla przemysłu\\\emph{semestr letni 2021/2022}}
\date{\today}
\begin{document}
	\section{autocorr}
	\begin{gather}
		\hat{\gamma}(h)=\frac{1}{n}\displaystyle{\sum_{i=1}^{n-h}{\left(X_t-\overline{X}\right)\left(X_{t+h}-\overline{X}\right)}}, \quad h\in\mathbb{N}\\
		\hat{\rho}(h)=\frac{\hat{\gamma}(h)}{\hat{\gamma}(0)}, \quad h\in\mathbb{N}
	\end{gather}
	\section{autocorr1}
	\begin{gather}
		Q_n(x)=\kappa\times\{|x_j-x_k|; j<k\}_{(\tau)}\\
		\hat{\gamma}_{Q_N}(h)=\frac{1}{4}\left[Q_{N-h}^2(u + v) - Q_{N-h}^2{(u-v})\right]\\
		\hat{\rho}(h)_{Q_N}=\frac{Q_{N-h}^2(u + v) - Q_{N-h}^2{(u-v})}{Q_{N-h}^2(u + v) + Q_{N-h}^2{(u-v})}
	\end{gather}
	\section{autocorr2}
	\begin{gather}
		\hat{\gamma}(h)_{Q_n}=\frac{1}{\sum_{t=1}^{n-h}{L_t^{(\alpha)}L_{t+h}^{(\alpha)}}}\left\{\displaystyle{\sum_{t=1}^{n-h}}\left(X_t-\overline{X}^{(\alpha)}\right)\left(X_{t+h}-\overline{X}^{(\alpha)}\right)L_t^{(\alpha)}L_{t+h}^{(\alpha)}\right\}
	\end{gather}
gdzie:
\begin{gather}
	\overline{X}^{(\alpha)}=\frac{1}{\sum_{t=1}^nL_t^{(\alpha)}}\displaystyle{\sum_{t=1}^n{X_tL_t^{(\alpha)}}}\\
	L_t^{(\alpha)}=\begin{cases}
		1,\quad & X_{(g)} < X_t < X_{(n-g+1)} \\
		0, \quad & \text{poza tym}
	\end{cases}
	g=\lfloor{\alpha\cdot n\rfloor},\quad\text{dla } 0\leq\alpha\leq0.5\\
	\hat{\rho}(h)=\frac{\hat{\gamma}(h)}{\hat{\gamma}(0)}
\end{gather}
\section{autocorr3}
\begin{gather}
	c=\frac{1}{\sum_{i=1}^nJ\left(\frac{R_i}{n+1}\right)^2},\\
	J(x) = \Phi^{-1}(x),\quad x\in(0, 1)\\
	\hat{\rho}(h)=c\displaystyle{\sum_{i=1}^{n-h}J\left(\frac{R_i}{n+1}\right)\cdot J\left(\frac{R_{i+h}}{n+1}\right)}
\end{gather}
$\Phi^{-1}$ \pauza dystrybuanta odwrotna rozkładu normalnego\\
$R_i$ \pauza $i${\dywiz}ta ranga w szeregu
\section{autocorr4}
\begin{gather}
	\hat{\rho}(h)=\frac{\text{med}{\left(\tilde{X_i}\tilde{X}_{1+h},\dots, \tilde{X}_{n-h}\tilde{X_n}\right)}}{\text{med}{\left(\tilde{X_1^2},\dots, \tilde{X_n^2}\right)}}
\end{gather}
\section{autocorr5}
\begin{gather}
	\hat{\rho}(h)=\frac{1}{(n-h)(n-h-1)}\displaystyle{\sum_{i>j}\text{sign}((X_i-X_j)(X_{i+h}-X_{j+h}))}
\end{gather}
\section{autocorr6}
\begin{gather}
	\hat{\rho}(h)=\frac{1}{n-h}\displaystyle{\sum_{i=1}^{n-h}\text{sign}((X_i-\hat\mu)(X_{i+h} - \hat\mu))}
\end{gather}
gdzie $\hat\mu$ to mediana szeregu $X$
\section{autocorr7}
\begin{equation}
	\Xi_{i, j}^{(k)}=\frac{\Gamma_{i, j}^{(k)}}{\sqrt{\Gamma_{i, i}^{(k)}\cdot\Gamma_{j, j}^{(k)}}}
\end{equation}

\begin{equation}
	\Gamma^{(k)}=\frac{Z_k'Z_k}{n}
\end{equation}

\begin{equation}
	Z'_k = \begin{bmatrix}
		\tilde X_1 & \tilde X_2 & \hdots & \tilde X_{k+1}& \hdots & \tilde X_n & 0 & \hdots & 0 \\
		0 & \tilde X_1 & \hdots & \tilde X_k & \hdots &\tilde X_{n-1} & \tilde X_n & \ddots & \vdots \\
		\vdots & \ddots & \ddots & \vdots & & \vdots & \vdots & \ddots & 0 \\
		0 & \hdots & 0 & \tilde X_1 & \hdots &\tilde X_{n-k} & \tilde X_{n-k+1} & \hdots & \tilde X_n
	\end{bmatrix}\in\mathbb{R}^{(k+1)\times(n+k)}
\end{equation}

\begin{equation}
	\tilde X_t=X_t - \overline{X}
\end{equation}

\begin{equation}
	\hat\rho(h)=\frac{1}{k-h+1}\displaystyle{\sum_{i=1}^{k-h+1}\hat\Xi^{(k)}_{i, i+h}}
\end{equation}
\section{autocorr8}
\begin{gather}
	\hat{\rho}(h)=\frac{\text{Var}(X_{t+h}+X_t) - \text{Var}(X_{t+h}-X_t)}{\text{Var}(X_{t+h}+X_t) + \text{Var}(X_{t+h}-X_t)}
\end{gather}
\section{autocorr9}
\begin{gather}
	\MAD=1.4826\cdot\text{med}\{|x_i-x_{\text{med}}|;i=1,\dots,n\}\\
	\hat{\rho}(h)=\frac{\MAD(X_{t+h}+X_t) - \MAD(X_{t+h}-X_t)}{\MAD(X_{t+h}+X_t) + \MAD(X_{t+h}-X_t)}
\end{gather}
\section{autocorr10}
\begin{gather}
	\IQR=0.7413\cdot(Q_3-Q_1)\\
	\hat{\rho}(h)=\frac{\IQR(X_{t+h}+X_t) - \IQR(X_{t+h}-X_t)}{\IQR(X_{t+h}+X_t) + \IQR(X_{t+h}-X_t)}
\end{gather}
\end{document}